x86model/Model/Decode.v
@@ -2074,7 +2074,11 @@ Definition SFENCE_p := "0000" $$ "1111" $$ "1010" $$ "1110" $$ "1111" $$
   Definition instr_grammars_seg_op_override := 
     CDQ_p :: CMOVcc_p :: CWDE_p :: DIV_p :: IDIV_p :: 
     MOVSX_p :: MOVZX_p :: MUL_p :: NOP_p :: 
-    ROL_p :: ROR_p :: SAR_p :: SHL_p :: SHLD_p :: SHR_p :: SHRD_p :: nil.
+    ROL_p :: ROR_p :: SAR_p :: SHL_p :: SHLD_p :: SHR_p :: SHRD_p ::
+   (* it turns out that MOVD can take the op_override prefix; not sure about
+      other MMX instrs *)
+    MOVD_p
+    :: nil.
 
   Definition prefix_grammar_seg_override :=
     option_perm segment_override_p @
@@ -2099,7 +2103,7 @@ Definition SFENCE_p := "0000" $$ "1111" $$ "1010" $$ "1110" $$ "1111" $$
     FSCALE_p :: 
     FSIN_p :: FSINCOS_p :: FSQRT_p :: FST_p :: (* FSTCW_p :: *) FSTENV_p :: FSTP_p :: FSUB_p :: FSUBP_p :: FSUBR_p :: FSUBRP_p ::FTST_p ::
     FUCOM_p :: FUCOMP_p :: FUCOMPP_p :: FUCOMI_p :: FUCOMIP_p :: FXAM_p :: FXCH_p :: FXTRACT_p :: FYL2X_p :: FYL2XP1_p :: FWAIT_p :: 
-    EMMS_p :: MOVD_p :: MOVQ_p :: PACKSSDW_p :: PACKSSWB_p :: PACKUSWB_p :: PADD_p :: PADDS_p :: PADDUS_p :: PAND_p :: PANDN_p :: PCMPEQ_p :: PCMPGT_p :: 
+    EMMS_p :: MOVQ_p :: PACKSSDW_p :: PACKSSWB_p :: PACKUSWB_p :: PADD_p :: PADDS_p :: PADDUS_p :: PAND_p :: PANDN_p :: PCMPEQ_p :: PCMPGT_p :: 
     PMADDWD_p :: PMULHUW_p :: PMULHW_p :: PMULLW_p :: POR_p :: PSLL_p :: PSRA_p :: PSRL_p :: PSUB_p :: PSUBS_p :: PSUBUS_p :: PUNPCKH_p :: PUNPCKL_p :: PXOR_p :: 
     ADDPS_p :: ADDSS_p :: ANDNPS_p :: ANDPS_p :: CMPPS_p :: CMPSS_p :: COMISS_p :: CVTPI2PS_p :: CVTPS2PI_p :: CVTSI2SS_p :: CVTSS2SI_p :: CVTTPS2PI_p :: CVTTSS2SI_p ::
     DIVPS_p :: DIVSS_p :: LDMXCSR_p :: MAXPS_p :: MAXSS_p :: MINPS_p :: MINSS_p :: MOVAPS_p :: MOVHLPS_p :: MOVLPS_p :: MOVMSKPS_p :: MOVSS_p :: MOVUPS_p :: MULPS_p ::
